pulse/share/steel/examples/pulse/CustomSyntax.fst
@@ -1,33 +1,52 @@
 module CustomSyntax
+module T = FStar.Tactics
 module PM = Pulse.Main
+open Steel.ST.Util 
+open Steel.ST.Reference
+open Steel.FractionalPermission
+open FStar.Ghost
+module U32 = FStar.UInt32
+open Pulse.Steel.Wrapper
+
 
 ```pulse
-fn fibonacci(n:nat)
-  requires emp
-  returns  _ : nat
-  ensures emp
- {
-   let mut i0 = 1;
-   let mut i1 = 1;
-   let mut ctr = 1;   
-   while (ctr < n) 
-   invariant exists (n:pos). (pts_to ctr n * pts_to i1 (fib_spec n) * pts_to i0 (fib_spec (n - 1)))
-   {
-      let tmp = i0;
-      i0 := i1;
-      i1 := (tmp + i0);
-      ctr := (ctr + 1)
-   };
-   i1
-}
-```
-
-```pulse
-fn add (x y: int)
-  requires (pts_to x a * pts_to y b)
-  returns r:int
-  ensures (pts_to x a * pts_to y b * pure (r == a + b))
+fn test_write_10 (x:(ref FStar.UInt32.t))
+                 (n:(erased FStar.UInt32.t))
+   requires (pts_to x full_perm n)
+   returns _ : unit
+   ensures  (pts_to x full_perm 0ul)
 {
-  (x + y)
+    x := 1ul;
+    x := 0ul
 }
 ```
+
+// fn fibonacci(n:nat)
+//   requires emp
+//   returns  _ : nat
+//   ensures emp
+//  {
+//    let mut i0 = 1;
+//    let mut i1 = 1;
+//    let mut ctr = 1;   
+//    while (ctr < n) 
+//    invariant b . exists (n:pos). (pts_to ctr n * pts_to i1 (fib_spec n) * pts_to i0 (fib_spec (n - 1)))
+//    {
+//       let tmp = i0;
+//       i0 := i1;
+//       i1 := (tmp + i0);
+//       ctr := (ctr + 1)
+//    };
+//    i1
+// }
+// ```
+
+// ```pulse
+// fn add (x y: int)
+//   requires (pts_to x a * pts_to y b)
+//   returns r:int
+//   ensures (pts_to x a * pts_to y b * pure (r == a + b))
+// {
+//   (x + y)
+// }
+// ```
